fstar/new/MLS.TreeSync.fst
@@ -57,26 +57,24 @@ let rec apply_path (#l:level_n) (#n:tree_size l) (#i:leaf_index n) (a:credential
 
 
 (** Create a blank path after modifying a leaf *)
-let rec blank_path (l:level_n) (n:tree_size l) (i:leaf_index n) (oc:option credential_t) : pathsync l n i =
+let rec blank_path (l:level_n) (n:tree_size l) (i:leaf_index n) (olp:option leaf_package_t) : pathsync l n i =
   if l = 0 then
-    match oc with
-    | None -> PLeaf None
-    | Some c -> PLeaf (Some (mk_initial_leaf_package c))
+    PLeaf olp
   else if n <= pow2 (l-1) then
-    PSkip _ (blank_path (l-1) n i oc)
+    PSkip _ (blank_path (l-1) n i olp)
   else
     let (|dir,j|) = child_index l i in
-    PNode None (blank_path (l-1) (if dir = Left then (pow2 (l-1)) else (n - (pow2 (l-1)))) j oc)
+    PNode None (blank_path (l-1) (if dir = Left then (pow2 (l-1)) else (n - (pow2 (l-1)))) j olp)
 
-let rec unmerged_path (#l:level_n) (#n:tree_size l) (leaf_index:leaf_index n) (t:treesync l n) (cred:credential_t): pathsync l n leaf_index =
+let rec unmerged_path (#l:level_n) (#n:tree_size l) (leaf_index:leaf_index n) (t:treesync l n) (lp:leaf_package_t): pathsync l n leaf_index =
   match t with
   | TLeaf (_, _) ->
-    PLeaf (Some (mk_initial_leaf_package cred))
-  | TSkip _ t' -> PSkip _ (unmerged_path leaf_index t' cred)
+    PLeaf (Some lp)
+  | TSkip _ t' -> PSkip _ (unmerged_path leaf_index t' lp)
   | TNode (_, onp) left right ->
     let (|dir, new_leaf_index|) = child_index l leaf_index in
     let (child, _) = order_subtrees dir (left, right) in
-    let path_next = unmerged_path new_leaf_index child cred in
+    let path_next = unmerged_path new_leaf_index child lp in
     match onp with
     | None ->
       PNode None path_next
@@ -85,27 +83,90 @@ let rec unmerged_path (#l:level_n) (#n:tree_size l) (leaf_index:leaf_index n) (t
         {np with np_unmerged_leafs = insert_sorted leaf_index np.np_unmerged_leafs}
       )) path_next
 
+// Helper functions to truncate the tree
+
+val is_tree_empty: #l:nat -> #n:tree_size l -> treesync l n -> bool
+let rec is_tree_empty #l #n t =
+  match t with
+  | TNode _ left right ->
+    is_tree_empty left && is_tree_empty right
+  | TSkip _ t' -> is_tree_empty t'
+  | TLeaf (_, Some _) -> false
+  | TLeaf (_, None) -> true
+
+val add_skips: #l:nat -> #n:tree_size l -> treesync l n -> (n_res:tree_size l{n_res <= n} & treesync l n_res)
+let rec add_skips #l #n t =
+  match t with
+  | TNode data left right ->
+    if is_tree_empty right then (
+      let (|n_res, left_res|) = add_skips left in
+      (|n_res, TSkip _ left_res|)
+    ) else (
+      let (|n_right_res, right_res|) = add_skips right in
+      (|pow2 (l-1) + n_right_res, TNode data left right_res|)
+    )
+  | TSkip _ t' ->
+    let (|n_res, t_res|) = add_skips t' in
+    (|n_res, TSkip () t_res|)
+  | TLeaf _ -> (|n, t|)
+
+val remove_root_skip: #l:nat -> #n:tree_size l -> treesync l n -> (l_res:nat{l_res <= l} & n_res:tree_size l_res{n_res == n} & treesync l_res n_res)
+let rec remove_root_skip #l #n t =
+  match t with
+  | TNode _ _ _ -> (|l, n, t|)
+  | TSkip _ t' ->
+    //`let` necessary for F* to see that l_res <= l-1 implies l_res <= l
+    let (|l_res, n_res, t_res|) = remove_root_skip t' in
+    (|l_res, n_res, t_res|)
+  | TLeaf _ -> (|l, n, t|)
+
+val canonicalize_tree: #l:nat -> #n:tree_size l -> treesync l n -> (l_res:nat{l_res <= l} & n_res:tree_size l_res{n_res <= n} & treesync l_res n_res)
+let canonicalize_tree #l #n t0 =
+  let (|_, t1|) = add_skips t0 in
+  let (|l_res, n_res, t_res|) = remove_root_skip t1 in
+  (|l_res, n_res, t_res|)
+
+// Helper functions to add leaf / extend the tree
+
+val find_empty_leaf: #l:nat -> #n:tree_size l -> treesync l n -> option (leaf_index n)
+let rec find_empty_leaf #l #n t =
+  match t with
+  | TNode _ left right -> (
+    match find_empty_leaf left, find_empty_leaf right with
+    | Some x, _ -> Some x
+    | None, Some x -> Some ((pow2 (l-1)) + x)
+    | None, None -> None
+  )
+  | TSkip _ t' -> find_empty_leaf t'
+  | TLeaf (_, Some _) -> None
+  | TLeaf (_, None) -> Some 0
+
+val mk_one_leaf_tree: l:nat -> credential_t -> Pure (treesync l 1) (requires True) (fun res -> Some? (find_empty_leaf res))
+let rec mk_one_leaf_tree l c =
+  if l = 0 then
+    TLeaf (c, None)
+  else
+    TSkip () (mk_one_leaf_tree (l-1) c)
+
+val add_one_leaf: #l:nat -> #n:tree_size l{n <> pow2 l} -> credential_t -> treesync l n -> Pure (treesync l (n+1)) (requires True) (fun res -> Some? (find_empty_leaf res))
+let rec add_one_leaf #l #n c t =
+  match t with
+  | TNode (nc, np) left right -> (
+    TNode (nc, np) left (add_one_leaf c right)
+  )
+  | TSkip _ t' ->
+    if n = pow2 (l-1) then
+      TNode (c, None) t' (mk_one_leaf_tree (l-1) c)
+    else
+      TSkip () (add_one_leaf c t')
+
+val add_one_level: #l:nat -> credential_t -> treesync l (pow2 l) -> Pure (treesync (l+1) ((pow2 l)+1)) (requires True) (fun res -> Some? (find_empty_leaf res))
+let add_one_level #l c t =
+  TNode (c, None) t (mk_one_leaf_tree l c)
+
 ///
 /// API
 ///
-
-(** Create an operation that modifies the group state *)
-val mk_operation: st:state_t -> actor:credential_t
-  -> i:index_t st -> p:pathsync st.st_levels st.st_treesize i
-  -> Tot (option operation_t)
-
-let mk_operation st actor i p =
-  match (membership st).[i], (PLeaf?.data p) with
-  | _ -> None
-  | Some mc, Some lp ->
-  if mc = lp.lp_credential then None
-  else
-    Some ({op_levels = st.st_levels;
-           op_treesize = st.st_treesize;
-           op_index = i;
-           op_actor = actor;
-           op_path = p;})
-
 
 (** Create a new group state *)
 val create: gid:nat -> sz:pos -> init:member_array_t sz
@@ -117,10 +178,11 @@ let create gid sz init =
   | Some actor,Some l ->
     let t = create_tree l sz actor init in
     let st = mk_initial_state gid l sz t in
-    Some ({st with st_initial_tree = t;
+    Some ({st with //st_initial_tree = t;
                    st_transcript = bytes_empty})
 
 
+(*
 (** Apply an operation to a state *)
 val apply: state_t -> operation_t
   -> Tot (option state_t)
@@ -131,33 +193,45 @@ let apply st op =
     let nt = apply_path op.op_actor st.st_tree op.op_path in
     Some ({ st with st_version = st.st_version + 1; st_tree = nt;
             st_transcript = Seq.snoc st.st_transcript op})
+*)
 
+val state_update_tree: #l:level_n -> #n:tree_size l -> state_t -> treesync l n -> state_t
+let state_update_tree #l #n st new_tree =
+  ({ st with
+    st_levels = l;
+    st_treesize = n;
+    st_version = st.st_version + 1;
+    st_tree = new_tree;
+    //st_transcript = Seq.snoc st.st_transcript op //TODO
+  })
 
-(** Add a new joiner *)
-val add: st:state_t -> actor:credential_t
-  -> i:index_t st -> joiner:credential_t
-  -> Tot (option (operation_t & state_t))
+val add: state_t -> credential_t -> leaf_package_t -> state_t
+let add st actor lp =
+  match find_empty_leaf st.st_tree with
+  | Some i ->
+    let p = unmerged_path i st.st_tree lp in
+    state_update_tree st (apply_path actor st.st_tree p)
+  | None ->
+    let new_l = if st.st_treesize = pow2 st.st_levels then st.st_levels+1 else st.st_levels in
+    let new_n = st.st_treesize+1 in
+    let augmented_tree: treesync new_l new_n =
+      if st.st_treesize = pow2 st.st_levels then
+        add_one_level actor st.st_tree
+      else
+        add_one_leaf actor st.st_tree
+    in
+    let i = Some?.v (find_empty_leaf augmented_tree) in
+    let p = unmerged_path i augmented_tree lp in
+    state_update_tree st (apply_path actor augmented_tree p)
 
-let add st actor i joiner =
-  let p = unmerged_path i st.st_tree joiner in
-  match mk_operation st actor i p with
-  | None -> None
-  | Some op ->
-  match apply st op with
-  | None -> None
-  | Some st' -> Some (op,st')
+val update: st:state_t -> credential_t -> leaf_package_t -> index_t st -> state_t
+let update st actor lp i =
+  let p = blank_path st.st_levels st.st_treesize i (Some lp) in
+  state_update_tree st (apply_path actor st.st_tree p)
 
-
-(** Remove a member *)
-val remove: st:state_t -> actor:credential_t -> i:index_t st
-  -> Tot (option (operation_t & state_t))
-
+val remove: st:state_t -> credential_t -> i:index_t st -> state_t
 let remove st actor i =
   let p = blank_path st.st_levels st.st_treesize i None in
-  match mk_operation st actor i p with
-  | None -> None
-  | Some op ->
-  match apply st op with
-  | None -> None
-  | Some st' -> Some (op,st')
-
+  let blanked_tree = (apply_path actor st.st_tree p) in
+  let (|_, _, reduced_tree|) = canonicalize_tree blanked_tree in
+  state_update_tree st reduced_tree
